save

UnitProJ/expressOS/August/INode.dfy
@@ -41,7 +41,6 @@ good()
 && (forall nd :: nd in spine ==> nd in footprint)
 && listCond(spine)
 && |spine| == |footprint|
-
 && (next != null ==> next.Valid())
 }
 
@@ -97,7 +96,7 @@ r.spine := [r] + spine;
 return r;
 }
 
-/*
+
 method append(d:Data) returns (lastNd:INode)
 requires Valid();
 
@@ -116,9 +115,11 @@ assert node.footprint !! footprint;
 var tmpNd := this;
 ghost var index := 0;
 
+assert V3();
+
 while(tmpNd.next != null)
 invariant tmpNd != null && tmpNd.Valid();
-invariant listCond(spine);
+invariant goodSeqCond(spine);
 invariant index == |this.footprint| - |tmpNd.footprint|;
 invariant tmpNd == spine[index];
 decreases tmpNd.footprint;
@@ -132,7 +133,9 @@ tmpNd.next := node;
 
 ghost var mySeq := spine + [node];
 
-//
+//assert goodSeqCond(mySeq[0..index]);
+///////////////////////////////////////////////
+/*
 while(index >= 0)
 invariant -1 <= index <= |mySeq| - 2;
 invariant listCond(mySeq);
@@ -140,8 +143,16 @@ invariant mySeq[index+1].Valid();
 invariant mySeq[|mySeq|-1].Valid();
 invariant mySeq[index+1].spine == mySeq[index+1..];
 invariant mySeq[|mySeq|-1].next == null;
+
+invariant goodSeqCond(mySeq[0..index]);
+invariant index < |mySeq| - 2 ==>
+mySeq[index].footprint == {mySeq[index]} + old(mySeq[index+1].footprint);
+invariant index == |mySeq| - 2 ==> mySeq[index].footprint == {mySeq[index]};
+
+invariant mySeq[index+1].footprint == 
+	old(mySeq[index+1].footprint) + {node};
 {
-updateCurIndex(mySeq, index);
+updateCurIndex(mySeq, index, mySeq[index].footprint - {mySeq[index]}, node);
 
 index := index - 1;
 }
@@ -151,8 +162,9 @@ assert seqV(mySeq);
 assert ValidLemma2();
 assert ValidLemma();
 return node;
-}
 */
+}
+
 
 
 
@@ -215,6 +227,17 @@ else (
 spine == [this] + next.spine 
 && footprint == {this} + next.footprint
 && next.ValidLemma2())
+}
+
+predicate V3()
+requires Valid();
+reads this, footprint;
+ensures V3();
+ensures goodSeqCond(spine);
+ensures forall i :: 0 <= i < |spine| ==> goodSeqCond(spine[0..i]);
+{
+if next == null then spine == [this]
+else good() && next.V3()
 }
 
 predicate allDiff(mySeq:seq<INode>)
@@ -281,21 +304,20 @@ else
 && validSeqLemma2(mySeq[1..]))
 )
 }
-
 */
 //===============================================
 
 
 ghost method updateCurIndex(mySeq:seq<INode>, index:int, 
-			oldFp:set<INode>, newNd:INode)
+			oldNxtFp:set<INode>, newNd:INode)
 
 requires 0 <= index <= |mySeq| - 2;
 requires listCond(mySeq);
 requires mySeq[index+1].Valid();
 requires mySeq[index+1].spine == mySeq[index+1..];
 
-requires mySeq[index].footprint == {mySeq[index]} + oldFp;
-requires mySeq[index+1].footprint == oldFp + {newNd};
+requires mySeq[index].footprint == {mySeq[index]} + oldNxtFp;
+requires mySeq[index+1].footprint == oldNxtFp + {newNd};
 
 modifies mySeq[index];
 
@@ -305,7 +327,7 @@ ensures mySeq[index].Valid();
 
 ensures mySeq[index].spine == mySeq[index..];
 
-ensures mySeq[index].footprint == {mySeq[index]} + oldFp + {newNd};
+ensures mySeq[index].footprint == old(mySeq[index].footprint) + {newNd};
 {
 mySeq[index].tailContents := [mySeq[index+1].data] + mySeq[index+1].tailContents;
 
